\chapter{Proofs by Induction}
\section{Simple Induction}
\begin{wrapfigure}{l}{4cm}
  \begin{center}
    \vskip -0.5cm
    \qrset{link, height=3cm}
    \qrcode{https://youtu.be/jOnZTWGpX_I}
    \vskip 0.25cm
    \href{https://youtu.be/jOnZTWGpX_I}{youtu.be/jOnZTWGpX\_I}
  \end{center}
  \vskip -1.5cm
\end{wrapfigure}
Let us consider a simple problem: what is bigger $2^n$ or $n$? In this chapter,
we are going to study the simplest way to prove that $2^n > n$ for all positive
integers $n$. First, let us check that it is true for small integers $n$.
\begin{flushright}
  \begin{tabular}{c | c | c | c | c | c | c | c | c}
    $n$   & 1 & 2 & 3 & 4  & 5  & 6  & 7   & 8   \\
    \hline
    $2^n$ & 2 & 4 & 8 & 16 & 32 & 64 & 128 & 256
  \end{tabular}
\end{flushright}
We may also note that $2^n$ is growing faster than $n$, so we expect that if
$2^n > n$ for small integers $n$, then it is true for all positive integers $n$.

In order to prove this statement formally, we use the following principle.
\begin{principle}[The Induction Principle]
  Let $P(n)$ be some statement about a positive integer $n$.
  Hence, $P(n)$ is true for every positive integer $n$ iff
  \begin{description}
    \item[base case:] $P(1)$ is true and
    \item[induction step:] $P(k) \implies P(k + 1)$ is true for all positive
      integers $k$.
  \end{description}
\end{principle}

Let us prove now the statement using this principle.
We define $P(n)$ be the statement that ``$2^n > n$''.
$P(1)$ is true since $2^1 > 1$. Let us assume now that $2^n > n$. Note that
$2^{n + 1} = 2 \cdot 2^n > 2n \ge n + 1$. Hence, we proved the induction step.

\begin{exercise}
  Prove that $(1 + x)^n \ge 1 + nx$ for all positive integers $n$ and real
  numbers $x \ge -1$.
\end{exercise}

\section{Changing the Base Case}
Let us consider functions $n^2$ and $2^n$.

\begin{center}
  \begin{tabular}{c | c | c | c | c | c | c | c | c}
    $n$   & 1 & 2 & 3 & 4  & 5  & 6  & 7   & 8   \\
    \hline
    $n^2$ & 1 & 4 & 9 & 16 & 25 & 36 & 49  & 64  \\
    $2^n$ & 2 & 4 & 8 & 16 & 32 & 64 & 128 & 256
  \end{tabular}
\end{center}
Note that $2^n$ is greater than $n^2$ starting from $5$. But without some trick
we can not prove this using induction since for $n = 3$ it is not true!

The trick is to use the statement $P(n)$ stating that $(n + 4)^2 < 2^{n + 4}$.
The base case when $n = 1$ is true.
Let us now prove the induction step. Assume that $P(k)$ is true i.e.
$(k + 4)^2 < 2^{k + 4}$. Note that $2(k + 4)^2 < 2^{k + 1 + 4}$ but
$(k + 5)^2 = k^2 + 10k + 25 \le 2k^2 + 16k + 32 = 2(k + 4)^2$.
Which implies that
$2^{k + 1 + 4} > (k + 5)^2$. So $P(k + 1)$ is also true.

In order to avoid this strange $+4$ we may change the base
case and use the following argument.

\begin{theorem}
\label{theorem:induction-shifted-base}
  Let $P(n)$ be some statement about an integer $n$.
  Hence, $P(n)$ is true for every integer $n > n_0$ iff
  \begin{description}
    \item[base case:] $P(n_0 + 1)$ is true and
    \item[induction step:] $P(k) \implies P(k + 1)$ is true for all
      integers $k > n_0$.
  \end{description}
\end{theorem}

Using this generalized induction principle we may prove that $2^n \ge n^2$ for
$n \ge 5$. The base case for $n = 4$ is true. The induction step is also true;
indeed let $P(k)$ be true i.e. $(k + 4)^2 < 2^{k + 4}$. Hence,
$2(k + 4)^2 < 2^{k + 1 + 4}$ but
$(k + 5)^2 = k^2 + 10k + 25 \le 2k^2 + 16k + 32 = 2(k + 4)^2$.

Let us now prove the theorem. Note that the proof is based on an idea similar
to the trick with $+4$, we just used.
\begin{proof}[Proof of \Cref{theorem:induction-shifted-base}]
  \begin{description}
    \item[$\Rightarrow$] If $P(n)$ is true for any $n > n_0$ it is also true
      for $n = n_0 + 1$ which implies the base case. Additionally, it true for
      $n = k + 1$ so the induction step is also true.
    \item[$\Leftarrow$] In this direction the proof is a bit harder. Let us
      consider a statement $Q(n)$ saying that $P(n + n_0)$ is true. Note that
      by the base case for $P$, $Q(1)$ is true; by the induction step for $P$
      we know that $Q(n)$ implies $P(n + 1)$. As a result, by the induction
      principle $Q(n)$ is true for all positive integers $n$. Which implies
      that $P(n)$ is true for all integers $n > n_0$.
  \end{description}
\end{proof}

\section{Inductive Definitions}

We may also define objects inductively. Let us consider the sum
$1 + 2 + \dots + n$ a line of dots indicating ``and so on'' which indicates the
definition by induction. In this case, a more precise notation is
$\sum_{i = 1}^n i$.

\begin{definition}
  Let $a(1)$, \dots, $a(n)$, \dots be a sequence of integers. Then
  $\sum_{i = 1}^n a(i)$ is defined inductively by the following
  statements:
  \begin{itemize}
    \item $\sum_{i = 1}^1 a(i) = a(1)$, and
    \item $\sum_{i = 1}^{k + 1} a(i) =
        \sum_{i = 1}^k a(i) + a(k + 1)$.
  \end{itemize}
\end{definition}

Let us prove that $\sum_{i = 1}^n i = \frac{n (n + 1)}{2}$.
Note that by definition $\sum_{i = 1}^1 i = 1$ and
$\frac{1 (1 + 1)}{2} = 1$; hence, the base case holds. Assume that
$\sum_{i = 1}^n i = \frac{n (n + 1)}{2}$. Note that
$\sum_{i = 1}^{n + 1} i = \sum_{i = 1}^n i + (n + 1)$ and by the
induction hypothesis $\sum_{i = 1}^n i = \frac{n (n + 1)}{2}$.
Hence, $\sum_{i = 1}^{n + 1} i = \frac{n (n + 1)}{2} + (n + 1) =
\frac{(n + 1)(n + 2)}{2}$.

\begin{exercise}
  Prove that $\sum_{i = 1}^n 2^i = 2^{n + 1} - 2$.
\end{exercise}

\section{Analysis of Algorithms with Cycles}

Induction is very useful for analysing algorithms using cycles. Let us extend
the example we considered in \Vref{section:simple-algorithm}.

Let us consider the following algorithm.
\begin{algorithm}
  \begin{algorithmic}[1]
    \Function{Max}{$a_1$, \dots, $a_n$}
      \State{$r \gets a_1$}
      \For{$i$ from $2$ to $n$}
        \If{$a_i > r$}
          \State{$r \gets a_i$}
        \EndIf
      \EndFor
      \State\Return{r}
    \EndFunction
  \end{algorithmic}
  \caption{The algorithm that finds the maximum element of $a_1$, \dots, $a_n$.}
\end{algorithm}
We prove that it is working correctly. First, we need to define $r_1$,
\dots, $r_n$ the value of $r$ during the execution of the algorithm.
It is easy to see that $r_1 = a_1$ and
$
  r_{i + 1} =
  \begin{cases}
    r_i & \text{if } r_i > a_{i + 1} \\
    a_{i + 1} & \text{otherwise}
  \end{cases}
$.
Secondly, we prove by induction that $r_i$ is the maximum of $a_1$, \dots,
$a_i$. It is clear that the base case for $i = 1$ is true. Let us prove the
induction step from $k$ to $k + 1$. By the induction hypothesis, $r_k$
is the maximum of $a_1$, \dots, $a_k$. We may consider two following cases.
\begin{itemize}
  \item If $r_k > a_{k + 1}$, then $r_{k + 1} = r_{k}$ is the maximum of $a_1$,
    \dots, $a_{k + 1}$ since $r_k$ is the maximum of $a_1$, \dots, $a_k$.
  \item Otherwise, $a_{k + 1}$ is greater than or equal to $a_1$, \dots, $a_k$, hence,
    $r_{k + 1} = a_{k + 1}$.
\end{itemize}

\begin{exercise}
  Show that line~6 in the following sorting algorithm executes
  $\frac{n (n + 1)}{2}$ times.
  \begin{algorithm}
    \begin{algorithmic}[1]
      \Function{SelectionSort}{$a_1$, \dots, $a_n$}
        \For{$i$ from $1$ to $n$}
          \State{$r \gets a_i$}
          \State{$\ell \gets i$}
          \For{$j$ from $i$ to $n$}
            \If{$a_j > r$}
              \State $r \gets a_j$
              \State $\ell \gets j$
            \EndIf
          \EndFor
          \State{Swap $a_i$ and $a_\ell$.}
        \EndFor
      \EndFunction
    \end{algorithmic}
    \caption{The algorithm is selection sort, it sorts $a_1$, \dots, $a_n$.}
  \end{algorithm}
\end{exercise}



\section{Strong Induction}

Sometimes $P(k)$ is not enough to prove $P(k + 1)$ and we need all the
statements $P(1)$, \dots, $P(k)$. In this case we may use the following
induction  principle.

\begin{theorem}[The Strong Induction Principle]
\label{theorem:strong-induction}
  Let $P(n)$ be some statement about positive integer $n$.
  Hence, $P(n)$ is true for every integer $n > n_0$ iff
  \begin{description}
    \item[base case:] $P(n_0 + 1)$ is true and
    \item[induction step:] If $P(n_0 + 1)$, \dots, $P(n_0 + k)$ are true, then
      $P(n_0 + k + 1)$ is also true for all positive integers $k$.
  \end{description}
\end{theorem}

Before we prove this theorem let us prove some properties of Fibonacci numbers
using this theorem. The Fibonacci numbers are defined as follows:
$f_0 = 0$, $f_1 = 1$, and $f_k = f_{k - 1} + f_{k - 2}$ for $k \ge 2$ (note
that they are also defined using strong induction since we use not only
$f_{k - 1}$ to define $f_k$).

\begin{theorem}[The Binet formula]
  The Fibonacci numbers are given by the following formula
  \[
      f_n = \frac{\alpha^n - \beta^n}{\sqrt{5}},
  \]
  where $\alpha = \frac{1 + \sqrt{5}}{2}$ and
  $\beta = \frac{1 - \sqrt{5}}{2}$.
\end{theorem}
\begin{proof}
  We use the strong induction principle to prove this statement with $n_0 = -1$.
  Let us first prove the base case,
  $\frac{(\alpha^0 - \beta^0)}{\sqrt{5}} = 0 = f_0$.
  We also need to prove the induction step.
  \begin{itemize}
    \item If $k = 1$, then $\frac{(\alpha^1 - \beta^1)}{\sqrt{5}} = 1 = f_1$.
    \item Otherwise, by the induction hypothesis,
      $f_k = \frac{\alpha^k - \beta^k}{\sqrt{5}}$ and
      $f_{k - 1} = \frac{\alpha^{k - 1} - \beta^{k - 1}}{\sqrt{5}}$.
      By the definition of the Fibonacci numbers $f_{k + 1} = f_k + f_{k - 1}$.
      Hence,
      \[
        f_{k + 1} = \frac{\alpha^k - \beta^k}{\sqrt{5}} +
        \frac{\alpha^{k - 1} - \beta^{k - 1}}{\sqrt{5}}.
      \]
      Note that it is enough to show that
      \begin{equation}
      \label{equation:binet}
        \frac{\alpha^{k + 1} - \beta^{k + 1}}{\sqrt{5}} =
        \frac{\alpha^k - \beta^k}{\sqrt{5}} +
        \frac{\alpha^{k - 1} - \beta^{k - 1}}{\sqrt{5}}.
      \end{equation}
      Note that it is the same as
      \[
        \frac{\alpha^{k + 1} - \alpha^k - \alpha^{k - 1}}{\sqrt{5}} =
        \frac{\beta^{k + 1} - \beta^k - \beta^{k - 1}}{\sqrt{5}}.
      \]
      Additionally, note that $\alpha$ and $\beta$ are roots of the equation
      $x^2 - x - 1 = 0$. Hence,
      $\alpha^{k + 1} - \alpha^k - \alpha^{k - 1} = \alpha^{k - 1}(\alpha^2 -
      \alpha - 1) = 0$ and
      $\beta^{k + 1} - \beta^k - \beta^{k - 1} =
      \beta^{k - 1}(\beta^2 - \beta - 1) = 0$. Which implies
      equality~(\ref{equation:binet}).
  \end{itemize}
\end{proof}

Now we are ready to prove the strong induction principle.
\begin{proof}[Proof of \Cref{theorem:strong-induction}]
  It is easy to see that if $P(n)$ is true for all $n > n_0$, then the base
  case and the induction steps are true. Let us prove that if the base case and
  the induction step are true, then $P(n)$ is true for all $n > n_0$.

  Let $Q(k)$ be the statement that $P(n_0 + 1)$, \dots, $P(n_0 + k)$ are true.
  Note that $Q(1)$ is true by the base case for $P$. Additionally, note that if
  $Q(k)$ is true, then $Q(k + 1)$ is also true, by the induction step for $P$.
  Hence, by the induction principle, $Q(k)$ is true for all positive integers
  $k$. Which implies that $P(n_0 + k)$ is true for all positive integers $k$.
\end{proof}

\section{Recursive Definitions}
Sometimes you wish to define objects using objects of the same form like in the
case of inductive definitions but you do not know how to enumerate them using
an integer parameter.

One example of such a situation is the definition of an arithmetic formula.
\begin{description}
  \item[base case:] $x_i$ is an arithmetic formula on the variables $x_1$,
    \dots, $x_n$ for all $i$; if $c$ is a real number, then $c$ is also
    an arithmetic formula on the variables $x_1$, \dots, $x_n$.
  \item[recursion step:] If $P$ and $Q$ are arithmetic formulas on the variables
    $x_1$, \dots, $x_n$, then $(P + Q)$ and $P \cdot Q$ are arithmetic formulas
    on the variables $x_1$, \dots, $x_n$.
\end{description}
Note that this definition implicitly states that any other expressions are not
arithmetic formulas.

We can define recursively the value of such a formula. Let $v_1$, \dots, $v_n$
be some integers.
\begin{description}
  \item[base cases:] $x_i\big\rvert_{x_1 = v_1, \dots, x_n = v_n} = v_i$; in
    other words, the value of the arithmetic formula $x_i$ is equal to $v_1$
    when $x_1 = v_1$, \dots, $x_n = v_n$; if $c$ is a real number, then
    $c\rvert_{x_1 = v_1, \dots, x_n = v_n} = c$.
  \item[recursion steps:] If $P$ and $Q$ are arithmetic formulas on the
    variables $x_1$, \dots, $x_n$, then
    \[
      (P + Q)\big\rvert_{x_1 = v_1, \dots, x_n = v_n} =
      P\big\rvert_{x_1 = v_1, \dots, x_n = v_n} +
      Q\big\rvert_{x_1 = v_1, \dots, x_n = v_n}
    \]
    and
    \[
      (P \cdot Q)\big\rvert_{x_1 = v_1, \dots, x_n = v_n} =
      P\big\rvert_{x_1 = v_1, \dots, x_n = v_n} \cdot
      Q\big\rvert_{x_1 = v_1, \dots, x_n = v_n}.
    \]
\end{description}

For example, $((x_1 + x_2) \cdot x_3)$ is clearly an arithmetic formula on the
variables $x_1$, \dots, $x_n$. One may expect the value of this formula with
$x_1 = 1$, $x_2 = 0$, and $x_3 = -1$ be equal to $-1$, let us check:
\begin{itemize}
  \item Note that
    \[
      \begin{array}{l}
        x_1\big\rvert_{x_1 = 1, x_2 = 0, x_3 = -1} = 1, \\
        x_2\big\rvert_{x_1 = 1, x_2 = 0, x_3 = -1} = 0\text{, and} \\
        x_3\big\rvert_{x_1 = 1, x_2 = 0, x_3 = -1} = -1.
      \end{array}
    \]
  \item Hence,
    \[
      (x_1 + x_2)\big\rvert_{x_1 = 1, x_2 = 0, x_3 = -1} = 1 + 0 = 1.
    \]
  \item Finally,
    \[
      ((x_1 + x_2) \cdot x_3)\big\rvert_{x_1 = 1, x_2 = 0, x_3 = -1} = 1 \cdot -
      1 = -1.
    \]
\end{itemize}


A special case of induction which called structural induction is the easiest way
to prove properties of recursively defined objects. The idea of this is similar
to the idea of strong induction:
\begin{itemize}
  \item first, we prove the statement for the base case,
  \item after that we prove the induction step, using the assumption that the
    statement is true for all the substructures (e.g. subformulas in the
    previous definition).
\end{itemize}
To illustrate this method, we prove the following theorem.

\begin{theorem}
  For any arithmetic formula $A$ on $x$, there is a polynomial
  $p$ such that $p(v) = A\big\rvert_{x = v}$ for any real value $v$.
\end{theorem}
\begin{proof}
  \begin{description}
    \item[base cases:] If $A = x_i$, then consider the polynomial $p(x) = x$;
      it is easy to see that $A\big\rvert_{x = v} = v = p(v)$.
      If $A = c$ where $c$ is a real number, then consider the constant
      polynomial  $p(x) = c$; it is easy to note that $A\big\rvert_{x = v} = c =
       p(v)$.
    \item[induction step:] We need to consider two cases. Consider the case when
      $A = B_1 + B_2$. By the induction hypothesis, there are polynomials $q_1$
      and $q_2$ such that $B_1\big\rvert_{x = v} = q_1(v)$ and
      $B_2\big\rvert_{x = v} = q_2(v)$ for all real numbers $v$.
      We define $p(x) = q_1(x) + q_2(x)$ (it is a polynomial since sum of
      two polynomials is a polynomial). It is obvious that
      $A\big\rvert_{x = v} = B_1\big\rvert_{x = v} + B_2\big\rvert_{x = v} =
      q_1(v) + q_2(v) = p(v)$.

      Another case is $A = B_1 \cdot B_2$. Again, by the induction hypothesis,
      there are polynomials $q_1$ and $q_2$ such that
      $B_1\big\rvert_{x = v} = q_1(v)$ and
      $B_2\big\rvert_{x = v} = q_2(v)$ for all real numbers $v$.
      We define $p(x) = q_1(x) \cdot q_2(x)$ (it is a polynomial since product of
      two polynomials is a polynomial). It is obvious that
      $A\big\rvert_{x = v} = B_1\big\rvert_{x = v} \cdot B_2\big\rvert_{x = v} =
      q_1(v) \cdot q_2(v) = p(v)$.
  \end{description}
\end{proof}

\begin{exercise}
  \begin{itemize}
    \item Define arithmetic formulas with devision and define their value (make sure
      that you handled divisions by $0$).

    \item Show that for any arithmetic formula with division $A$ on $x$,
      there are polynomials $p$ and $q$ such that $\frac{p(v)}{q(v)} =
      A\big\rvert_{x = v}$ or $A\big\rvert_{x = v}$ is not defined for
      any real value $v$.
  \end{itemize}
\end{exercise}


\section{Analysis of Recursive Algorithms}
To illustrate the power of recursive definitions and strong induction, let us
analyze \Cref{algorithm:binary-search}.
\begin{algorithm}
  \begin{algorithmic}[1]
    \Function{BinarySearch}{$e$, $a_1$, \dots, $a_n$}
      \If{$n \le 5$}
        \For{$i$ from $1$ to $n$}
          \If{$a_i = e$}
            \State\Return{i}
          \EndIf
        \EndFor
      \Else
        \State{$\ell \gets \floor{\frac{n}{2}}$}
        \If{$a_\ell \le e$}
          \State\Call{BinarySearch}{$e$, $a_1$, \dots, $a_\ell$}
        \Else
          \State\Call{BinarySearch}{$e$, $a_{\ell + 1}$, \dots, $a_n$}
        \EndIf
      \EndIf
    \EndFunction
  \end{algorithmic}
  \caption{The binary search algorithm that finds an element $e$ in the sorted
    list $a_1$, \dots, $a_n$.}
  \label{algorithm:binary-search}
\end{algorithm}
We prove that number of comparisons of this algorithm is bounded by
$6 + 2\log_2(n)$. First step of the proof is to denote the worst
number of comparisons when we run the algorithm on the list of length $n$ by
$C(n)$. It is easy to see that $C(n) = n$ for $n \le 5$. Additionally,
$C(n) \le 1 + \max(C(\floor{\frac{n}{2}}), C(n - \floor{\frac{n}{2}}))$ for
$n > 5$. As we mentioned we prove that $C(n) \le 6 + 2\log_2(n)$, we prove it
by induction. The base case is clear; let us now prove the induction step.
By the induction hypothesis,
\[
  C(\floor{\frac{n}{2}}) \le 6 + 2\log_2(\floor{\frac{n}{2}})
\]
and
\[
  C(n - \floor{\frac{n}{2}}) \le 6 + 2\log_2(n - \floor{\frac{n}{2}}).
\]
Since $\floor{\frac{n}{2}} \le \frac{n}{2}$ and $n - \floor{\frac{n}{2}} \le
\frac{n}{2} + 1$, $C(n) \le 1 + 2\log_2(\frac{n}{2} + 1)$.
However,
\[
  1 + 6 + 2\log_2\left(\frac{n}{2} + 1\right) \le
  6 + 2\log_2\left(\frac{n}{\sqrt{2}} + \sqrt{2}\right) \le 6 + 2 \log_2(n)
\]
for $n \ge 5$. As a result, we proved the induction step.

\section*{End of The Chapter Exercises}
\begin{exercises}
  \exerciseitem Show that there does not exist the largest integer.
  \exerciseitem Show that for any positive integer $n$, $n^2 + n$ is even.
  \exerciseitem Show that for any positive integer $n$, $3$ divises
    $n^3 + 2n$.
  \exerciseitem Show that for any integer $n \ge 10$,
    $n^3 \le 2^n$.
  \exerciseitem Show that for any positive integer $n$,
    $\sum_{i = 0}^n x^i = \frac{1 - x^{n + 1}}{1 - x}$.
  \exerciseitem Show that for any matrix $A \in \mathbb{R}^{m \times n}$
    ($n > m$) there is a nonzero vector $x \in \mathbb{R}^n$ such that $Ax = 0$.
  \exerciseitem  Show that all the elements of $\set{0, 1}^n$ (Binary strings)
    may be ordered such that every successive strings in this order are
    different only in one character.
    (For example, for $n = 2$ the order may be $00$, $01$, $11$, $10$.)
  \exerciseitem Let $a_0 = 2$, $a_1 = 5$, and $a_n = 5a_{n - 1} - 6 a_{n - 2}$
    for all integers $n \ge 2$. Show that $a_n = 3^n + 2^n$ for all integers
    $n \ge 0$.
  \exerciseitem Show that $\sum_{i = 1}^n i^2 = \frac{n (n + 1)(2n + 1)}{6}$
    for all integers $n \ge 1$.
  \exerciseitem Show that $\sum\limits_{i = 1}^n \frac{1}{i (i + 1)} =
    \frac{n}{n + 1}$ for all integers $n \ge 1$.
  \exerciseitem Show that $\sum\limits_{i = 1}^n \frac{1}{i^2} \le
    2 - \frac{1}{n}$ for all integers $n \ge 1$.
  \exerciseitem Show that $\sum_{i = 1}^n (2i - 1) = n^2$ for any positive
    integer $n$.
  \exerciseitem Prove that $\sum_{i = 1}^n \frac{1}{i (i + 1)} =
    \frac{n}{n + 1}$ for any positive integer $n$.
  \exerciseitem Prove that $\sum\limits_{i = 2}^n (i + 1) 2^i = n 2^{n + 1}$
    for all integers $n > 2$.
  \exerciseitem Let $a_1$, \dots, $a_n$ be a sequence of real numbers.
    We define inductively
    $\prod_{i = k}^n a_i$ as follows:
    \begin{itemize}
      \item $\prod_{i = 1}^1 a_i = a_1$ and
      \item $\prod_{i = 1}^{k + 1} a_i =
        \left( \prod_{i = 1}^k a_i \right) \cdot a_{k + 1}$.
      \end{itemize}

      Prove that $\prod_{i = 1}^{n - 1} \left(1 - \frac{1}{(i + 1)^2} \right) =
      \frac{n + 1}{2n}$ for all integers $n > 1$.

  \exerciseitem Let $f_0 = 1$, $f_1 = 1$, and $f_{n + 2} = f_{n + 1} + f_n$ for
    all $n \in \mathbb{N}$. Show that
    $f_n \ge \left(\frac{3}{2}\right)^{n - 2}$.
  \exerciseitem Show that $f_{n + m} = f_{n - 1} f_m + f_n f_{m + 1}$.
  \exerciseitem Show that two arithmetic formulas $(x_1 + x_2) \cdot x_3$ and
    $x_1 \cdot x_3 + x_2 \cdot x_3$ on the variables $x_1$, $x_2$, and $x_3$
    have the same values.

  \exerciseitem We say that $L$ is a list of powers of $x$ iff
    \begin{itemize}
      \item either $L = x^k$ for some positive integer $k$ or
      \item $L = (x^k, L')$ where $L'$ is a list of powers of $x$ and
        $k$ is a positive integer.
    \end{itemize}

    Let $L$ be a list of powers of $x$. We say that the sum of $L$
    with $x = v$ denoted by $\sum L\big\rvert_{x = v}$
    \begin{itemize}
      \item is equal to $x^k$ whether $L = x^k$ and
      \item is equal to $x^k + \sum L'\big\rvert_{x = v}$ whether
        $L = (x^k, L')$.
    \end{itemize}

    Prove that for any list $L$ of powers of $x$ there is a polynomial such that
    $\sum L\big\rvert_{x = v} = p(v)$ for all real numbers $v$.

\end{exercises}
